More work in ByteStringFMap.v

src/ByteStringFMap.v
@@ -41,7 +41,7 @@ Variable heap : Rep HSpec.
    proof word that is done in HeapFMap.v). *)
 
 Record PS' := {
-  ps'Heap : ComputationalADT.cRep (projT1 HeapImpl);
+  ps'Heap : Rep HeapSpec;
 
   ps'Buffer : N;
   ps'BufLen : N;
@@ -50,9 +50,179 @@ Record PS' := {
   ps'Length : N
 }.
 
-Variable heap' : ComputationalADT.cRep (projT1 HeapImpl).
-Variable AbsR : Heap_AbsR (` heap) heap'.
+(* Strip away the proofy bits. *)
+Lemma ByteStringStrip :
+  { adt : _ & refineADT (projT1 (ByteStringHeap heap)) adt }.
+Proof.
+  eexists.
+  hone representation using
+       (fun (or : PS) (nr : PS') =>
+          ` (psHeap or) = ps'Heap nr /\
+          psBuffer or = ps'Buffer nr /\
+          psBufLen or = ps'BufLen nr /\
+          psOffset or = ps'Offset nr /\
+          psLength or = ps'Length nr);
+  try simplify with monad laws; simpl.
+  {
+    refine pick val {| ps'Heap   := ` heap
+                     ; ps'Buffer := 0
+                     ; ps'BufLen := 0
+                     ; ps'Offset := 0
+                     ; ps'Length := 0 |}.
+      finish honing.
+    simpl; intuition.
+  }
+  {
+    repeat match goal with
+      [ H : _ /\ _ |- _ ] => destruct H
+    end; subst.
+    rewrite H1, H2, H3, H4.
+    rewrite refineEquiv_If_Then_Else_Bind.
+    apply refine_If_Then_Else.
+      simplify with monad laws; simpl.
+      unfold poke'; simpl.
+      remove_dependency; simpl.
+      rewrite H0.
+      etransitivity.
+        apply refine_under_bind; intros.
+        refine pick val {| ps'Heap   := fst a
+                         ; ps'Buffer := ps'Buffer r_n
+                         ; ps'BufLen := ps'BufLen r_n
+                         ; ps'Offset := ps'Offset r_n - 1
+                         ; ps'Length := ps'Length r_n + 1 |}.
+          simplify with monad laws.
+          finish honing.
+        intuition.
+      simpl.
+      finish honing.
+    rewrite refineEquiv_If_Then_Else_Bind.
+    subst H.
+    apply refine_If_Then_Else.
+      simplify with monad laws; simpl.
+      unfold memcpy', poke'; simpl.
+      remove_dependency; simpl.
+      setoid_rewrite refine_bind_dep_bind_ret; simpl.
+      do 2 setoid_rewrite refine_bind_dep_ignore.
+      etransitivity.
+        apply refine_under_bind; intros.
+        etransitivity.
+          apply refine_under_bind; intros.
+          refine pick val {| ps'Heap   := fst a0
+                           ; ps'Buffer := ps'Buffer r_n
+                           ; ps'BufLen := ps'BufLen r_n
+                           ; ps'Offset := 0
+                           ; ps'Length := ps'Length r_n + 1 |}.
+            simplify with monad laws.
+            finish honing.
+          intuition.
+        simpl.
+        finish honing.
+      simpl.
+      rewrite H0.
+      finish honing.
+    rewrite refineEquiv_If_Then_Else_Bind.
+    apply refine_If_Then_Else.
+      simplify with monad laws; simpl.
+      unfold alloc', memcpy', poke'.
+      remove_dependency; simpl.
+      do 3 setoid_rewrite refine_bind_dep_bind_ret.
+      simpl; remove_dependency.
+      do 3 setoid_rewrite refine_bind_dep_ignore.
+      unfold ByteStringHeap.buffer_cons_obligation_2.
+      rewrite H0.
+      etransitivity.
+        apply refine_under_bind; intros.
+        etransitivity.
+          apply refine_under_bind; intros.
+          etransitivity.
+            apply refine_under_bind; intros.
+            etransitivity.
+              apply refine_under_bind; intros.
+              refine pick val {| ps'Heap   := fst a2
+                               ; ps'Buffer := snd a
+                               ; ps'BufLen := ps'Length r_n +1
+                               ; ps'Offset := 0
+                               ; ps'Length := ps'Length r_n + 1 |}.
+                simplify with monad laws.
+                finish honing.
+              intuition.
+            simpl; finish honing.
+          simpl; finish honing.
+        simpl; finish honing.
+      simpl; finish honing.
+    unfold allocate_buffer, alloc', poke'.
+    simplify with monad laws; simpl.
+    remove_dependency; simpl.
+    setoid_rewrite refine_bind_dep_ret.
+    autorewrite with monad laws; simpl.
+    remove_dependency.
+    rewrite H0.
+    unfold ByteStringHeap.buffer_cons_obligation_3.
+    etransitivity.
+      apply refine_under_bind; intros.
+      remember (Map _ _) as M.
+      refine pick val {| ps'Heap   := M
+                       ; ps'Buffer := snd a
+                       ; ps'BufLen := 1
+                       ; ps'Offset := 0
+                       ; ps'Length := 1 |}.
+        simplify with monad laws.
+        rewrite HeqM.
+        finish honing.
+      intuition.
+    simpl.
+    finish honing.
+  }
+  {
+    repeat match goal with
+      [ H : _ /\ _ |- _ ] => destruct H
+    end; subst.
+    rewrite H1, H2, H3, H4.
+    rewrite refineEquiv_If_Then_Else_Bind.
+    subst H.
+    apply refine_If_Then_Else.
+      simplify with monad laws; simpl.
+      unfold peek'.
+      remove_dependency.
+      rewrite H0.
+      etransitivity.
+        apply refine_under_bind; intros.
+        refine pick val {| ps'Heap   := ps'Heap r_n
+                         ; ps'Buffer := ps'Buffer r_n
+                         ; ps'BufLen := ps'BufLen r_n
+                         ; ps'Offset := if ps'Length r_n =? 1
+                                        then 0
+                                        else ps'Offset r_n + 1
+                         ; ps'Length := ps'Length r_n - 1 |}.
+          simplify with monad laws.
+          finish honing.
+        intuition.
+      simpl.
+      finish honing.
+    simplify with monad laws; simpl.
+    rewrite H0.
+    refine pick val r_n.
+      simplify with monad laws; simpl.
+      finish honing.
+    intuition.
+  }
+  apply reflexivityT.
+Defined.
 
+Record CPS := {
+  cpsHeap : ComputationalADT.cRep (projT1 HeapImpl);
+
+  cpsBuffer : N;
+  cpsBufLen : N;
+
+  cpsOffset : N;
+  cpsLength : N
+}.
+
+Variable cheap : ComputationalADT.cRep (projT1 HeapImpl).
+Variable AbsR : Heap_AbsR (` heap) cheap.
+
+(*
 Lemma refine_pick_PS' : forall P a b c d,
   refine {r_n0 : PS' | P (ps'Heap r_n0) /\
                        a = ps'Buffer r_n0 /\
@@ -67,128 +237,47 @@ Lemma refine_pick_PS' : forall P a b c d,
                         d = ps'Length r_n0}).
 Proof.
 Admitted.
+*)
 
-(* Strip away the proofy bits. *)
-Lemma ByteStringStrip :
-  { adt : _ & refineADT (projT1 (ByteStringHeap heap)) adt }.
+Lemma ByteStringFMap :
+  { adt : _ & refineADT (projT1 ByteStringStrip) adt }.
 Proof.
   eexists.
   hone representation using
-       (fun (or : PS) (nr : PS') =>
-          Heap_AbsR (` (psHeap or)) (ps'Heap nr) /\
-          psBuffer or = ps'Buffer nr /\
-          psBufLen or = ps'BufLen nr /\
-          psOffset or = ps'Offset nr /\
-          psLength or = ps'Length nr);
+       (fun (or : PS') (nr : CPS) =>
+          Heap_AbsR (ps'Heap or) (cpsHeap nr) /\
+          ps'Buffer or = cpsBuffer nr /\
+          ps'BufLen or = cpsBufLen nr /\
+          ps'Offset or = cpsOffset nr /\
+          ps'Length or = cpsLength nr);
   try simplify with monad laws; simpl.
   {
-    refine pick val {| ps'Heap   := heap'
-                     ; ps'Buffer := 0
-                     ; ps'BufLen := 0
-                     ; ps'Offset := 0
-                     ; ps'Length := 0 |}.
+    refine pick val {| cpsHeap   := cheap
+                     ; cpsBuffer := 0
+                     ; cpsBufLen := 0
+                     ; cpsOffset := 0
+                     ; cpsLength := 0 |}.
       finish honing.
-    simpl; intuition.
+    intuition.
   }
   {
     repeat match goal with
       [ H : _ /\ _ |- _ ] => destruct H
     end; subst.
-    rewrite H1; clear H1.
-    rewrite H2; clear H2.
-    rewrite H3; clear H3.
-    rewrite H4; clear H4.
+    rewrite H1, H2, H3, H4.
     rewrite refineEquiv_If_Then_Else_Bind.
     apply refine_If_Then_Else.
-      simplify with monad laws; simpl.
-      unfold poke'; simpl.
-      remove_dependency; simpl.
-      etransitivity.
-        apply refine_under_bind; intros.
-        rewrite refine_pick_PS'.
-        simplify with monad laws.
-        finish honing.
-      simpl.
-      rewrite
-        (Heap_refine_poke
-           H0 _ _
-           (fun u =>
-              r_n' <- { r_n0 : PS' |
-                        fst u             = ps'Heap   r_n0 /\
-                        ps'Buffer r_n     = ps'Buffer r_n0 /\
-                        ps'BufLen r_n     = ps'BufLen r_n0 /\
-                        ps'Offset r_n - 1 = ps'Offset r_n0 /\
-                        ps'Length r_n + 1 = ps'Length r_n0 };
-              ret (r_n', ()))).
-        remember (M.mapi _ _) as M.
-        refine pick val
-          {| ps'Heap   := (fst (ps'Heap r_n), M)
-           ; ps'Buffer := ps'Buffer r_n
-           ; ps'BufLen := ps'BufLen r_n
-           ; ps'Offset := ps'Offset r_n - 1
-           ; ps'Length := ps'Length r_n + 1 |}.
-          simplify with monad laws.
-          rewrite HeqM.
-          finish honing.
-        simpl; intuition.
-      exact (proj2_sig (psHeap r_o)).
+      admit.
     rewrite refineEquiv_If_Then_Else_Bind.
     subst H.
     apply refine_If_Then_Else.
       simplify with monad laws; simpl.
-      unfold memcpy', poke'; simpl.
-      remove_dependency; simpl.
-      setoid_rewrite refine_bind_dep_bind_ret; simpl.
-      do 2 setoid_rewrite refine_bind_dep_ignore.
-      setoid_rewrite refine_pick_PS'.
-      etransitivity.
-        apply refine_under_bind; intros.
-        etransitivity.
-          apply refine_under_bind; intros.
-          simplify with monad laws.
-          finish honing.
-        simpl.
-        finish honing.
-      simpl.
-      rewrite N.add_0_r.
-(*
-      rewrite
-        (Heap_refine_poke
-           _ _ _
-           (fun u =>
-              r_n' <- {r_n0 : PS' |
-                       fst u             = ps'Heap   r_n0 /\
-                       ps'Buffer r_n     = ps'Buffer r_n0 /\
-                       ps'BufLen r_n     = ps'BufLen r_n0 /\
-                       0                 = ps'Offset r_n0 /\
-                       ps'Length r_n + 1 = ps'Length r_n0};
-              ret (r_n', ()))).
-
-        rewrite Heap_refine_poke.
-      setoid_rewrite refine_bind_dep_ret; simpl.
-      remove_dependency.
-      simplify with monad laws; simpl.
-*)
       admit.
     rewrite refineEquiv_If_Then_Else_Bind.
     apply refine_If_Then_Else.
       simplify with monad laws; simpl.
-      unfold alloc', memcpy', poke'.
-      remove_dependency.
-      do 3 setoid_rewrite refine_bind_dep_bind_ret.
-      simpl; remove_dependency.
-      do 3 setoid_rewrite refine_bind_dep_ignore.
-      unfold ByteStringHeap.buffer_cons_obligation_2.
-      erewrite Heap_refine_alloc'; eauto.
-        admit.
-      exact (proj2_sig (psHeap r_o)).
-    unfold allocate_buffer, alloc', poke'.
+      admit.
     simplify with monad laws; simpl.
-    remove_dependency.
-    setoid_rewrite refine_bind_dep_ret.
-    autorewrite with monad laws; simpl.
-    remove_dependency.
-    unfold ByteStringHeap.buffer_cons_obligation_3.
     admit.
   }
   {
@@ -200,9 +289,6 @@ Proof.
     subst H.
     apply refine_If_Then_Else.
       simplify with monad laws; simpl.
-      unfold peek'.
-      remove_dependency.
-      destruct (psHeap r_o); simpl in *; subst.
       admit.
     simplify with monad laws; simpl.
     refine pick val r_n.
